docs/sbft-formal-model/replica.i.dfy
@@ -79,6 +79,11 @@ module Replica {
     {
       map seqID | seqID in getActiveSequenceIDs(c) :: if seqID in m then m[seqID] else empty
     }
+    function Clear<T>(c:Constants, m:map<SequenceID,T>, empty:T) : map<SequenceID,T> 
+      requires c.WF()
+    {
+      map seqID | seqID in getActiveSequenceIDs(c) :: empty
+    }
   }
 
 
@@ -189,14 +194,60 @@ module Replica {
          else highestOfRest
   }
 
+  function ExtractSeqIDsFromPrevView(c:Constants, v:Variables, newViewMsg:Network.Message<Message>) : set<SequenceID>
+    requires c.WF()
+    requires v.WF(c)
+    requires newViewMsg.payload.NewViewMsg?
+    requires newViewMsg.payload.valid(c.clusterConfig.AgreementQuorum())
+    requires newViewMsg in v.newViewMsgsRecvd.msgs
+    // readability:
+    requires newViewMsg.payload.newView == v.view
+    requires CurrentPrimary(c, v) == newViewMsg.sender
+    requires LiteInv(c, v)
+  {
+    // 1. Check Each VC Msg for correct proof for last stable SeqID.
+    // 2. Check New View for containing only correct VC msgs. 
+    // 3. Get the highest SeqID form the VC msgs and if seqID is within the previous View's WW compute restrictions, otherwise return None
+
+    if v.view == 0 
+    then {}
+    else
+      var vcMsgs:set := newViewMsg.payload.vcMsgs.msgs;
+      var highestStable := HighestStable(c, vcMsgs);
+      set seqID:SequenceID | && WithinRange(c, highestStable, seqID) // This statement provides a trigger by naming the constraint
+                             && highestStable < seqID <= highestStable + c.clusterConfig.workingWindowSize // This statement satisfies Dafny's finite set heuristics.
+  }
+
+  predicate WithinRange(c:Constants, highestStable:SequenceID, seqID:SequenceID)
+  {
+    highestStable < seqID <= highestStable + c.clusterConfig.workingWindowSize
+  }
+
+  function HighestStable(c:Constants, msgs:set<Network.Message<Message>>) : SequenceID
+    requires c.WF()
+    requires forall m | m in msgs :: m.payload.ViewChangeMsg?
+  {
+    if |msgs| == 0
+    then 1
+    else
+      var vcMsg :| vcMsg in msgs;
+      var rest := msgs - {vcMsg};
+      if vcMsg.payload.lastStableCheckpoint > HighestStable(c, rest)
+      then vcMsg.payload.lastStableCheckpoint
+      else HighestStable(c, rest)
+  }
+
   function CalculateRestrictionForSeqID(c:Constants, v:Variables, seqID:SequenceID, newViewMsg:Network.Message<Message>) 
     : Option<OperationWrapper>
       requires v.WF(c)
       requires newViewMsg.payload.NewViewMsg?
       requires newViewMsg.payload.vcMsgs.valid(v.view, c.clusterConfig.AgreementQuorum())
+      requires newViewMsg in v.newViewMsgsRecvd.msgs
       // readability:
       requires newViewMsg.payload.newView == v.view
       requires CurrentPrimary(c, v) == newViewMsg.sender
+      requires seqID in v.workingWindow.getActiveSequenceIDs(c)
+      requires LiteInv(c, v)
     {
     // 1. Take the NewViewMsg for the current View.
     // 2. Go through all the ViewChangeMsg-s in the NewView and take the valid full 
@@ -205,18 +256,22 @@ module Replica {
     // 4. If it is empty  we need to fill with NoOp.
     // 5. If it contains valid full quorum we take the Client Operation and insist it will be committed in the new View.
 
-    var relevantPrepareCertificates := set viewChangeMsg, cert |
-                                   && viewChangeMsg in newViewMsg.payload.vcMsgs.msgs
-                                   && cert == viewChangeMsg.payload.certificates[seqID]
-                                   && cert.WF()
-                                   && !cert.empty()
-                                     :: cert;
-    if |relevantPrepareCertificates| == 0
-    then
-      Some(Noop)
+    if seqID !in ExtractSeqIDsFromPrevView(c, v, newViewMsg)
+    then None
     else
-      var highestViewCert := HighestViewPrepareCertificate(relevantPrepareCertificates);
-      Some(highestViewCert.prototype().operationWrapper)
+      var relevantPrepareCertificates := set viewChangeMsg, cert |
+                                     && viewChangeMsg in newViewMsg.payload.vcMsgs.msgs
+                                     && seqID in viewChangeMsg.payload.certificates
+                                     && cert == viewChangeMsg.payload.certificates[seqID]
+                                     && cert.WF()
+                                     && !cert.empty()
+                                       :: cert;
+      if |relevantPrepareCertificates| == 0
+      then
+        Some(Noop)
+      else
+        var highestViewCert := HighestViewPrepareCertificate(relevantPrepareCertificates);
+        Some(highestViewCert.prototype().operationWrapper)
   }
 
   predicate ViewIsActive(c:Constants, v:Variables) {
@@ -440,17 +495,29 @@ module Replica {
     // Change messages for in viewChangeMsgsRecvd or View is 0.
     && (|| (HasCollectedProofMyViewIsAgreed(c, v) && newView == v.view + 1)
         || HaveSufficientVCMsgsToMoveTo(c, v, newView))
-    && var vcMsg := Network.Message(c.myId, ViewChangeMsg(newView, ExtractCertificatesFromWorkingWindow(c, v)));
-    && (forall seqID :: seqID in vcMsg.payload.certificates ==> 
-               (vcMsg.payload.certificates[seqID].valid(c.clusterConfig.AgreementQuorum())))
+    && var vcMsg := Network.Message(c.myId, 
+                                    ViewChangeMsg(
+                                      newView,
+                                      v.workingWindow.lastStableCheckpoint,
+                                      CheckpointsQuorum(ExtractStableCheckpointProof(c, v)),
+                                      ExtractCertificatesFromWorkingWindow(c, v)));
+    // TODO: this should follow from the invariant and from the way we collect prepares. Might be put in LiteInv.
+    // && (forall seqID :: seqID in vcMsg.payload.certificates ==> 
+    //            (vcMsg.payload.certificates[seqID].valid(c.clusterConfig.AgreementQuorum())))
     && v' == v.(view := newView)
               .(viewChangeMsgsRecvd := v.viewChangeMsgsRecvd.(msgs := v.viewChangeMsgsRecvd.msgs + {vcMsg}))
   }
 
-  function ExtractCertificatesFromWorkingWindow(c:Constants, v:Variables) : imap<SequenceID, PreparedCertificate> //TODO refactor after Checkpoint is added.
+  function ExtractStableCheckpointProof(c:Constants, v:Variables) : set<Network.Message<Message>>
     requires v.WF(c)
   {
-    imap seqID | seqID in v.workingWindow.preparesRcvd :: ExtractCertificateForSeqID(c, v, seqID)
+    set msg | msg in v.checkpointMsgsRecvd.msgs && msg.payload.seqIDReached == v.workingWindow.lastStableCheckpoint
+  }
+
+  function ExtractCertificatesFromWorkingWindow(c:Constants, v:Variables) : map<SequenceID, PreparedCertificate>
+    requires v.WF(c)
+  {
+    map seqID | seqID in v.workingWindow.getActiveSequenceIDs(c) :: ExtractCertificateForSeqID(c, v, seqID)
   }
 
   function ExtractCertificateForSeqID(c:Constants, v:Variables, seqID:SequenceID) : PreparedCertificate
@@ -511,6 +578,7 @@ module Replica {
     && (forall seqID | seqID in msg.payload.certificates
             :: && msg.payload.certificates[seqID].votes <= msgOps.signedMsgsToCheck
                && msg.payload.certificates[seqID].valid(c.clusterConfig.AgreementQuorum()))
+    && msg.payload.valid(c.clusterConfig.AgreementQuorum())
     && v' == v.(viewChangeMsgsRecvd := v.viewChangeMsgsRecvd.(msgs := v.viewChangeMsgsRecvd.msgs + {msg}))
   }
 
@@ -524,10 +592,16 @@ module Replica {
     && msg.payload.newView == v.view
     && msg.payload.vcMsgs.msgs <= msgOps.signedMsgsToCheck
     // Check that all the PreparedCertificates are valid
-    && msg.payload.vcMsgs.valid(v.view, c.clusterConfig.AgreementQuorum())
+    && msg.payload.valid(c.clusterConfig.AgreementQuorum())
     // We only allow the primary to select 1 set of View Change messages per view.
     && (forall storedMsg | storedMsg in v.newViewMsgsRecvd.msgs :: msg.payload.newView != storedMsg.payload.newView)
-    && v' == v.(newViewMsgsRecvd := v.newViewMsgsRecvd.(msgs := v.newViewMsgsRecvd.msgs + {msg}))
+    && assert (forall m | m in msg.payload.vcMsgs.msgs :: m.payload.ViewChangeMsg?);
+       v' == v.(newViewMsgsRecvd := v.newViewMsgsRecvd.(msgs := v.newViewMsgsRecvd.msgs + {msg}))
+              .(workingWindow := v.workingWindow.(
+                lastStableCheckpoint := HighestStable(c, msg.payload.vcMsgs.msgs), 
+                prePreparesRcvd := v.workingWindow.Clear(c, v.workingWindow.prePreparesRcvd, None),
+                preparesRcvd := v.workingWindow.Clear(c, v.workingWindow.preparesRcvd, EmptyPrepareProofSet()),
+                commitsRcvd := v.workingWindow.Clear(c, v.workingWindow.commitsRcvd, EmptyCommitProofSet())))
   }
 
   predicate SendCheckpoint(c:Constants, v:Variables, v':Variables, msgOps:Network.MessageOps<Message>, seqID:SequenceID) {
